theories/language/weakestpre.v
@@ -54,9 +54,9 @@ Definition wp_pre `{!melocotonGS_gen hlc val pubstate Λ Σ}
     (∀ σ ns, state_interp σ ns ={E}=∗
       (  (∃ v, ⌜e = of_class Λ (ExprVal v)⌝ ∗ state_interp σ ns ∗ Φ v)
        ∨ (∃ s vv K, ⌜e = fill K (of_class Λ (ExprCall s vv))⌝ ∗ ⌜p !! s = None⌝ ∗
-            ▷ |={E}=> (state_interp σ (S ns) ∗ ∃ Ξ, T s vv Ξ ∗ ∀ r, Ξ r -∗ wp E (fill K (of_class Λ (ExprVal r))) Φ))
-       ∨ ((⌜reducible p e σ⌝ ∗
-                    ∀ σ' e', ⌜prim_step p e σ e' σ' []⌝ -∗ |={E}=> ▷ |={E}=> 
+          |={E}=> ▷ |={E}=> (∃ σ'  Ξ, state_interp σ' (S ns) ∗ T s vv Ξ ∗ ∀ r, Ξ r -∗ wp E (fill K (of_class Λ (ExprVal r))) Φ))
+       ∨ ((⌜reducible_no_threads p e σ⌝ ∗
+                    ∀ σ' e', ⌜prim_step p e σ e' σ' []⌝ -∗  |={E}=> ▷ |={E}=> 
                         (state_interp σ' (S ns) ∗ wp E e' Φ)))))%I.
 
 Local Instance wp_pre_contractive `{!melocotonGS_gen hlc val pubstate Λ Σ}
@@ -100,11 +100,11 @@ Global Instance wp_ne pe E e n :
 Proof.
   revert e. induction (lt_wf n) as [n _ IH]=> e Φ Ψ HΦ.
   rewrite !wp_unfold /wp_pre /=.
-  do 15 f_equiv. 1: f_equiv.
+  do 15 f_equiv. 1: do 2 f_equiv.
   all: f_contractive.
   all: f_equiv.
   all: f_equiv. 
-  1: do 4 f_equiv; intros r; f_equiv. 
+  1: do 2 f_equiv; intros r; do 5 f_equiv. 
   all: apply IH; eauto; intros k; eapply dist_le', HΦ; lia.
 Qed.
 Global Instance wp_proper pe E e :
@@ -137,7 +137,7 @@ Qed.
 
 Definition prog_environ_mono pe1 pe2 : Prop := 
    prog pe1 = prog pe2
-/\ ∀ (s:string) vv Φ, T pe1 s vv Φ -∗ T pe2 s vv Φ.
+/\ ∀ (s:string) vv Φ, ⌜s ∉ (dom (prog pe1))⌝ -∗ T pe1 s vv Φ -∗ T pe2 s vv Φ.
 
 Lemma prog_environ_mono_refl : Reflexive (prog_environ_mono).
 Proof. intros s; split; eauto. Qed.
@@ -151,28 +151,32 @@ Proof.
   rewrite !wp_unfold /wp_pre /=.
   iIntros "%σ %ns Hσ". iSpecialize ("H" $! σ ns with "Hσ").
   iMod (fupd_mask_subseteq E1) as "Hclose"; first done.
-  iMod "H". iMod "Hclose".
-  iDestruct "H" as "[(%x & -> & Hσ & H)|[(%s & %vv & %K & -> & H2 & H3)|H3]]".
-  - iLeft. iExists x. iFrame. iSplitR; first done. 
+  iMod "H".
+  iDestruct "H" as "[(%x & -> & Hσ & H)|[(%s & %vv & %K & -> & %H2 & H3)|H3]]".
+  - iMod "Hclose". iLeft. iExists x. iFrame. iSplitR; first done. 
     iApply ("HΦ" with "[> -]"). by iApply (fupd_mask_mono E1 _); first apply HE.
-  - iRight; iLeft. iExists s, vv, K. iSplitR; first done. rewrite Hpe1; iFrame.
-    do 2 iModIntro.
+  - iRight; iLeft. iExists s, vv, K. iMod "Hclose".
     iMod (fupd_mask_subseteq E1) as "Hclose2"; first done.
     iMod "H3".
-    iMod "Hclose2". iModIntro.
-    iDestruct "H3" as "(Hσ & %Ξ & HT & Hr)".
-    iFrame. iExists Ξ. iSplitL "HT"; first iApply (Hpe2 s vv with "HT").
+    iMod "Hclose2".  iModIntro. iSplitR; first done. iSplitR; first (iPureIntro; congruence).
+    do 2 iModIntro.
+    iMod (fupd_mask_subseteq E1) as "Hclose2'"; first done.
+    iMod "H3". iMod "Hclose2'". iModIntro.
+    iDestruct "H3" as "(%σ' & %Ξ & Hσ & HT & Hr)".
+    iFrame. iExists σ', Ξ. iFrame. iSplitL "HT"; first iApply (Hpe2 s vv with "[] HT").
+    1: iPureIntro; by apply not_elem_of_dom_2.
     iIntros "%r HΞ". iApply ("IH" $! (fill K (of_class Λ (ExprVal r))) E1 E2 HE Φ Ψ with "[Hr HΞ] HΦ").
     iApply ("Hr" with "HΞ").
   - do 2 iRight. 
     iDestruct "H3" as "(HH & H3)".
-    iModIntro. rewrite Hpe1. iFrame. iIntros "%σ2 %e' Hstep".
+    rewrite Hpe1.  iMod "Hclose". iFrame. iModIntro. iIntros "%σ2 %e' Hstep".
     iSpecialize ("H3" $! σ2 e' with "Hstep").
-    iMod (fupd_mask_subseteq E1) as "Hclose2"; first done.
-    iMod "H3". iMod "Hclose2". iModIntro. iModIntro.
-    iMod (fupd_mask_subseteq E1) as "Hclose3"; first done.
-    iMod "H3" as "(Hσ & HWP)". iMod "Hclose3".
-    iModIntro. iFrame. iApply ("IH" $! e' E1 E2 HE Φ Ψ with "HWP HΦ").
+    iMod (fupd_mask_subseteq E1) as "Hclose2"; first done. iMod "H3".
+    iMod "Hclose2". iModIntro. iModIntro.
+    iMod (fupd_mask_subseteq E1) as "Hclose2'"; first done.
+    iMod "H3" as "(Hσ & HWP)".
+    iMod "Hclose2'". iModIntro.
+    iFrame. iApply ("IH" $! e' E1 E2 HE Φ Ψ with "HWP HΦ").
 Qed.
 
 Lemma fupd_wp pe E e Φ : (|={E}=> WP e @ pe; E {{ Φ }}) ⊢ WP e @ pe; E {{ Φ }}.
@@ -222,16 +226,16 @@ Proof.
   iMod ("Hwp" $! σ1 ns with "Hσ") as "[(%z & -> & Hσ & H)|[(%s & %vv & %K & -> & H2 & H3)|(%Hred & H3)]]".
   + unfold to_val in Heq. rewrite to_of_class in Heq.
     exfalso. apply TCEq_eq in Heq. congruence.
-  + cbn. iRight. iLeft. iMod "HP". iModIntro.
-    iExists s, vv, K. iFrame. iSplitR; first done.
-    iModIntro. iMod "HP". iMod "HP". iMod "H3" as "(Hσ & %Ξ & Hvv & HΞ)". iModIntro. iFrame.
-    iExists Ξ. iFrame. iIntros "%r Hr". iSpecialize ("HΞ" $! r with "Hr").
+  + cbn. iRight. iLeft. iMod "HP". iMod "H3".
+    iExists s, vv, K. iFrame. iSplitR; first done. do 3 iModIntro.
+    iMod "HP". iMod "HP". iMod "H3" as "(%σ'& %Ξ & Hσ & Hvv & HΞ)". iModIntro. iFrame.
+    iExists σ', Ξ. iFrame. iIntros "%r Hr". iSpecialize ("HΞ" $! r with "Hr").
     iApply (wp_strong_mono pe pe E E with "HΞ [HP]"). 1-2:easy.
     iIntros "%v Hv". iMod ("Hv" with "HP"). iAssumption.
   + iMod "HP". iModIntro. iRight. iRight. iSplitR; first done.
-    iIntros "%σ' %e' %Hstep". iSpecialize ("H3" $! σ' e' Hstep).
-    iMod "H3". do 2 iModIntro. iMod "H3" as "(Hσ' & H3)". do 2 iMod "HP".
-    iModIntro; iFrame.
+    iIntros "%σ' %e' %Hstep". iSpecialize ("H3" $! σ' e' Hstep). iMod "H3". iModIntro. iModIntro.
+    iMod "H3" as "(Hσ' & H3)". do 2 iMod "HP". iModIntro.
+    iFrame.
     iApply (wp_strong_mono pe pe E E with "H3 [HP]"). 1-2:easy.
     iIntros "%v Hv". iMod ("Hv" with "HP"). iAssumption.
 Qed.
@@ -278,41 +282,61 @@ Proof.
     iMod ("H" $! σ ns with "Hσ") as "H". iApply "H".
   - iRight. iLeft. iExists s, vv, (comp_ectx K K').
     iFrame. iSplitR.
-    {iModIntro; iPureIntro. now rewrite fill_comp. }
-    do 2 iModIntro. iMod "H3" as "(Hσ & %Ξ & HT & Hr)". iModIntro. iFrame.
-    iExists Ξ. iFrame.
+    {iModIntro; iPureIntro. now rewrite fill_comp. } iMod "H3".
+    do 3 iModIntro. iMod "H3" as "(%σ'& %Ξ & Hσ & HT & Hr)". iModIntro. iFrame.
+    iExists σ', Ξ. iFrame.
     iIntros "%r HΞ".
     rewrite <- fill_comp.
     iApply "IH". iApply ("Hr" with "HΞ").
   - iRight. iRight. iModIntro. iDestruct "H3" as "(%Hred & H3)".
-    iSplitR; first eauto using reducible_fill.
+    iSplitR; first eauto using reducible_no_threads_fill.
     iIntros "%σ' %e' %Hstep".
-    pose proof (reducible_not_val _ _ _ Hred) as  Hnone.
+    pose proof (reducible_not_val _ _ _ (reducible_no_threads_reducible _ _ _ K Hred)) as  Hnone.
     destruct (fill_step_inv _ _ _ _ _ _ _ Hnone Hstep) as (e2'' & -> & H4).
-    iSpecialize ("H3" $! σ' e2'' H4).
-    iMod "H3". iModIntro. iModIntro.
+    iSpecialize ("H3" $! σ' e2'' H4). iMod "H3". do 2 iModIntro.
     iMod "H3" as "(Hσ & H3)". iModIntro. iFrame.
     iApply "IH". iApply "H3".
 Qed.
 
-(*
+(* TODO: extract this lemma into language.v *)
 Lemma wp_bind_inv K s E e Φ :
+  (forall K K' e s' vv, fill K e = fill K' (of_class Λ (ExprCall s' vv)) -> (exists K'', K' = comp_ectx K K'') \/ is_Some (to_val e)) ->
   WP fill K e @ s; E {{ Φ }} ⊢ WP e @ s; E {{ v, WP fill K (of_class _ (ExprVal v)) @ s; E {{ Φ }} }}.
 Proof.
-  iIntros "H". iLöb as "IH" forall (E e Φ). do 2 rewrite {1} wp_unfold /wp_pre /=.
+  intros Hassum. iIntros "H".
+  iLöb as "IH" forall (E e Φ). do 2 rewrite {1} wp_unfold /wp_pre /=.
+  assert ((exists v, e = of_val _ v) \/ (forall v, e <> of_val _ v)) as [[v Hv]|Hnv].
+  1: { destruct (to_val e) as [v|] eqn:Heq.
+       + left. exists v. now apply of_to_val in Heq.
+       + right. intros v ->. rewrite to_of_val in Heq. congruence. }
+  1: { rewrite Hv.
+       iIntros "%σ %ns Hσ". iModIntro. iLeft. iExists v. iFrame. iSplitR; first done.
+       rewrite {1} wp_unfold /wp_pre /=. iApply "H". }
   iIntros "%σ %ns Hσ".
-  iMod ("H" $! σ ns with "Hσ") as "[(%x & %H1 & Hσ & H)|[(%s' & %vv & %K' & H1 & H2 & H3)|H3]]".
-  - destruct (fill_class' K e) as [->|(v&<-%of_to_class)].
+  iMod ("H" $! σ ns with "Hσ") as "[(%x & %H1 & Hσ & H)|[(%s' & %vv & %K' & %H1 & %H2 & H3)|(%Hred & H3)]]".
+  - destruct (fill_class' K e) as [->|[v Hv]].
     + eexists. rewrite H1. now rewrite to_of_class.
-    + rewrite ! fill_empty in H1. subst. iLeft.
-      iModIntro. iExists _. iSplitR; first done. rewrite fill_empty. iFrame.
-      rewrite {1} wp_unfold /wp_pre /=. iIntros "%σ' %ns' Hσ'".
-      iModIntro. iLeft. iExists x. iFrame. done.
-    + iLeft. iExists v. iModIntro. iSplitR; first done.
-      iFrame. rewrite H1.
-      rewrite {1} wp_unfold /wp_pre /=. iIntros "%σ' %ns' Hσ'".
-      iModIntro. iLeft. iExists x. iFrame. done.
-  - *)
+    + rewrite fill_empty in H1. exfalso. eapply Hnv. apply H1.
+    + apply of_to_class in Hv. exfalso. eapply Hnv. rewrite <- Hv. easy.
+  - destruct (Hassum _ _ _ _ _ H1) as [[K'' ->]|[x Hx]].
+    + rewrite <- fill_comp in H1. apply fill_inj in H1. subst.
+      iRight. iLeft. iExists s', vv, K''. iMod "H3".
+      iModIntro. iSplitR; first done. iSplitR; first done.
+      do 2 iModIntro. iMod "H3" as "(%σ'& %Ξ & Hσ & HT & Hr)".
+      iModIntro. iExists σ', Ξ. iFrame.
+      iIntros (r) "HΞr".
+      iApply "IH". rewrite fill_comp. by iApply "Hr".
+    + unfold to_val in Hx. destruct (to_class e) as [[v|]|] eqn:Heq; try congruence.
+      exfalso. eapply Hnv. apply of_to_class in Heq. rewrite <- Heq. easy.
+  - iModIntro.
+    iRight. iRight. iSplitR. 1: iPureIntro.
+    { destruct Hred as (e'&σ'&(e''&->&H2)%fill_step_inv). 1: by eexists e'',σ'.
+      destruct (to_val e) eqn:Heq; try congruence. exfalso. apply (Hnv v). apply of_to_val in Heq. done. }
+    iIntros (σ' e' Hred').
+    iSpecialize ("H3" $! σ' _ (fill_prim_step _ K e _ _ _ _ Hred')). iMod "H3". do 2 iModIntro.
+    iMod "H3" as "(Hσ & HWP)". iModIntro. iFrame.
+    iApply "IH". iFrame.
+Qed.
 
 (** * Derived rules *)
 Lemma wp_mono pe E e Φ Ψ : (∀ v, Φ v ⊢ Ψ v) → WP e @ pe; E {{ Φ }} ⊢ WP e @ pe; E {{ Ψ }}.
@@ -400,6 +424,92 @@ Proof.
   iIntros "HR HWP". iApply (wp_wand with "HWP").
   iIntros (v) "HΦ". by iApply "HΦ".
 Qed.
+(*
+Lemma wp_link s1 s2 k E e Φ :
+  (forall K K' e s' vv, fill K e = fill K' (of_class Λ (ExprCall s' vv)) -> (exists K'', K' = comp_ectx K K'') \/ is_Some (to_val e)) ->
+  ⌜(prog s2 = delete k (prog s1))⌝
+  -∗ (□ ((∀ (s:string) vv Ψ, ⌜s ∉ (dom (prog s2))⌝ -∗ T s1 s vv Ψ -∗ T s2 s vv Ψ)
+         ∗ (∀ vv Ψ, WP (of_class Λ (ExprCall k vv)) @ s1; E {{v, Ψ v}} -∗ T s2 k vv Ψ)))
+  -∗ WP e @ s1; E {{v, Φ v}}
+  -∗ WP e @ s2; E {{v, Φ v}}.
+Proof.
+  intros Hassum.
+  iIntros (HE) "#(Hs2T & Hs1T) H". iLöb as "IH" forall (e Φ).
+  rewrite !wp_unfold /wp_pre /=.
+  iIntros "%σ %ns Hσ". iSpecialize ("H" $! σ ns with "Hσ").
+  iMod "H".
+  iDestruct "H" as "[(%x & -> & Hσ & H)|[(%s & %vv & %K & -> & %H2 & H3)|(%HH & H3)]]".
+  - iLeft. iExists x. iFrame. iModIntro. done.
+  - iRight; iLeft. iExists s, vv, K. iSplitR; first done. iSplitR; 
+    first (iPureIntro; rewrite HE; apply lookup_delete_None; by right).
+    iModIntro. iMod "H3". do 2 iModIntro.
+    iMod "H3" as "(%σ' & %Ξ & Hσ & HT & Hr)". iModIntro.
+    iFrame. iExists σ',Ξ. iFrame. iSplitL "Hs1T HT"; first iApply ("Hs2T" $! s vv with "[] HT").
+    1: iPureIntro; apply not_elem_of_dom_2; rewrite HE; apply lookup_delete_None; by right.
+    iIntros "%r HΞ". iApply ("IH" $! (fill K (of_class Λ (ExprVal r))) Φ).
+    iApply ("Hr" with "HΞ").
+  - destruct HH as (e' & σ' & (K & e1' & e2' & -> & -> & Hhead)%prim_step_inv).
+    destruct (to_class e1') as [[v|kk]|] eqn:Heq.
+    + apply val_head_stuck in Hhead.
+      unfold to_val in Hhead. rewrite Heq in Hhead. congruence.
+    + iRight. destruct (string_dec kk k) as [->|Hne].
+      * iLeft. iExists k, arg, K.
+        iDestruct ("H3" $! σ' (fill K e2') (Prim_step _ K _ _ _ _ _ _ _ eq_refl eq_refl Hhead)) as "H3'".
+        iModIntro. iSplitR; last iSplitR.
+        1: iPureIntro; apply of_to_class in Heq; by rewrite Heq.
+        1: rewrite HE; iPureIntro; apply lookup_delete. do 2 iModIntro.
+        iMod "H3'" as "(Hσ & HWP)".
+        iModIntro. iFrame. iExists σ'.
+        iExists (λ r, WP fill K (of_class Λ (ExprVal r)) @ s2; E {{ v, Φ v }})%I.
+        iFrame. iSplitL. 2: iIntros (r) "Hr"; iApply "Hr".
+        iApply "Hs1T".
+        rewrite (wp_unfold s1 E (of_class Λ (ExprCall k arg))).
+        unfold wp_pre.
+        iIntros "%σp %nsp Hσp". iRight. iRight. iModIntro.
+        apply of_to_class in Heq. rewrite <-Heq in Hhead.
+        iSplitR.
+        {iPureIntro. exists e2',σp. eapply head_prim_step, head_call_pure, Hhead. }
+        iIntros (σp' e' Hstep2). iModIntro. iMod (state_interp_mono with "Hσp") as "Hσp". iModIntro.
+        assert (σp = σp' /\ e2' = e') as [-> ->].
+        { apply head_reducible_prim_step in Hstep2.
+          1: eapply call_head_step in Hstep2; destruct Hstep2 as (fn & Hfn & He' & -> & _);
+             eapply call_head_step in Hhead; destruct Hhead as (fn' & Hfn' & He2 & -> & _); split; congruence.
+          eapply head_call_pure in Hhead. do 3 eexists. apply Hhead. }
+        iFrame. iApply (wp_wand with "[HWP]"). 2: { iIntros (v) "Hv". iApply "IH". iApply "Hv". }
+        iApply wp_bind_inv. 1: easy. iApply "HWP".
+      * iRight. iModIntro. assert (head_step (prog s2) e1' σ e2' σ []) as Hstep'. 
+        { apply of_to_class in Heq. subst e1'. apply call_head_step in Hhead.
+          apply call_head_step. destruct Hhead as (fn & H1 & H2 & H3 & H4). exists fn. repeat try split; try done.
+          rewrite HE. rewrite lookup_delete_ne. 1: apply H1. congruence. } 
+        iSplitR.
+        {iPureIntro. do 2 eexists. apply fill_prim_step. apply head_prim_step. done. }
+        iIntros (σ'1 e'1 Hstep).
+        assert (prim_step (prog s1) (fill K e1') σ (e'1) σ'1 []) as Hprim. 
+        { apply fill_reducible_prim_step in Hstep. 2: do 3 eexists; apply head_prim_step; exact Hstep'.
+          destruct Hstep as (e'' & -> & Hprim).
+          apply head_reducible_prim_step in Hprim. 2: do 3 eexists; exact Hstep'.
+          apply of_to_class in Heq. subst e1'. apply call_head_step in Hprim.
+          apply fill_prim_step. apply head_prim_step.
+          apply call_head_step. destruct Hprim as (fn & H1 & H2 & H3 & H4). exists fn. repeat try split; try done.
+          rewrite HE in H1. Search lookup delete. rewrite lookup_delete_ne in H1. 1: apply H1. congruence. } 
+        iSpecialize ("H3" $! _ _ Hprim).
+        iModIntro. iMod "H3" as "(Hσ' & HWP')". iModIntro. iFrame.
+        iApply "IH". iApply "HWP'".
+  + iRight. iRight. iModIntro. i
+ iApply 
+ iFrame.
+        1: iApply (state_interp_mono with "Hσp").
+
+
+ do 2 iRight. 
+    iDestruct "H3" as "(HH & H3)".
+    iModIntro. rewrite Hpe1. iFrame. iIntros "%σ2 %e' Hstep".
+    iSpecialize ("H3" $! σ2 e' with "Hstep").
+    iMod (fupd_mask_subseteq E1) as "Hclose2"; first done.
+    iMod "H3". iMod "Hclose2". iModIntro. iModIntro.
+    iMod (fupd_mask_subseteq E1) as "Hclose3"; first done.
+    iMod "H3" as "(Hσ & HWP)". iMod "Hclose3".
+    iModIntro. iFrame. iApply ("IH" $! e' E1 E2 HE Φ Ψ with "HWP HΦ"). *)
 End wp.
 
 (** Proofmode class instances *)
