theories/ml_toy_lang/melocoton/primitive_laws.v
@@ -6,15 +6,15 @@ From iris.bi.lib Require Import fractional.
 From iris.base_logic.lib Require Import mono_nat.
 From iris.base_logic.lib Require Export gen_heap proph_map gen_inv_heap.
 From melocoton.language Require Export weakestpre lifting.
-From melocoton.c_toy_lang Require Export melocoton.class_instances.
-From melocoton.c_toy_lang Require Import tactics melocoton.tactics notation.
+From melocoton.ml_toy_lang Require Export melocoton.class_instances.
+From melocoton.ml_toy_lang Require Import melocoton.tactics notation.
 From iris.prelude Require Import options.
 
 Class heapGS_gen hlc Σ := HeapGS {
   heapGS_invGS : invGS_gen hlc Σ;
-  heapGS_gen_heapGS :> gen_heapGS loc heap_cell Σ;
-  heapGS_inv_heapGS :> inv_heapGS loc heap_cell Σ;
-  heapGS_proph_mapGS :> proph_mapGS positive (prod val val) Σ;
+  heapGS_gen_heapGS :> gen_heapGS loc val Σ;
+  heapGS_inv_heapGS :> inv_heapGS loc val Σ;
+  heapGS_proph_mapGS :> proph_mapGS proph_id (val * val) Σ;
   heapGS_step_name : gname;
   heapGS_step_cnt : mono_natG Σ;
 }.
@@ -59,6 +59,7 @@ Section steps.
 
 End steps.
 
+
 Global Program Instance heapGS_melocotonGS `{heapGS_gen hlc Σ} 
       : melocotonGS_gen hlc val state (C_lang_melocoton) Σ := {
   iris_invGS := heapGS_invGS;
@@ -70,88 +71,48 @@ Next Obligation.
   by iMod (steps_auth_update_S with "H") as "$".
 Qed.
 
-(** Since we use an [option val] instance of [gen_heap], we need to overwrite
+(** Since we use an [val] instance of [gen_heap], we need to overwrite
 the notations.  That also helps for scopes and coercions. *)
 (** FIXME: Refactor these notations using custom entries once Coq bug #13654
 has been fixed. *)
-
-Notation "l O↦{ dq } v" := (mapsto (L:=loc) (V:=heap_cell) l dq (v))
-  (at level 20, format "l  O↦{ dq }  v") : bi_scope.
-Notation "l O↦□ v" := (mapsto (L:=loc) (V:=heap_cell) l DfracDiscarded (v))
-  (at level 20, format "l  O↦□  v") : bi_scope.
-Notation "l O↦{# q } v" := (mapsto (L:=loc) (V:=heap_cell) l (DfracOwn q) (v))
-  (at level 20, format "l  O↦{# q }  v") : bi_scope.
-Notation "l O↦ v" := (mapsto (L:=loc) (V:=heap_cell) l (DfracOwn 1) (v))
-  (at level 20, format "l  O↦  v") : bi_scope.
-
-Notation "l I↦{ dq } v" := (mapsto (L:=loc) (V:=heap_cell) l dq (Some v))
-  (at level 20, format "l  I↦{ dq }  v") : bi_scope.
-Notation "l I↦□ v" := (mapsto (L:=loc) (V:=heap_cell) l DfracDiscarded (Some v))
-  (at level 20, format "l  I↦□  v") : bi_scope.
-Notation "l I↦{# q } v" := (mapsto (L:=loc) (V:=heap_cell) l (DfracOwn q) (Some v))
-  (at level 20, format "l  I↦{# q }  v") : bi_scope.
-Notation "l I↦ v" := (mapsto (L:=loc) (V:=heap_cell) l (DfracOwn 1) (Some v))
-  (at level 20, format "l  I↦  v") : bi_scope.
-
-Notation "l ↦{ dq } v" := (mapsto (L:=loc) (V:=heap_cell) l dq (Some (Some v%V)))
+Notation "l ↦{ dq } v" := (mapsto (L:=loc) (V:=val) l dq (v%V))
   (at level 20, format "l  ↦{ dq }  v") : bi_scope.
-Notation "l ↦□ v" := (mapsto (L:=loc) (V:=heap_cell) l DfracDiscarded (Storing v%V))
+Notation "l ↦□ v" := (mapsto (L:=loc) (V:=val) l DfracDiscarded (v%V))
   (at level 20, format "l  ↦□  v") : bi_scope.
-Notation "l ↦{# q } v" := (mapsto (L:=loc) (V:=heap_cell) l (DfracOwn q) (Storing v%V))
+Notation "l ↦{# q } v" := (mapsto (L:=loc) (V:=val) l (DfracOwn q) (v%V))
   (at level 20, format "l  ↦{# q }  v") : bi_scope.
-Notation "l ↦ v" := (mapsto (L:=loc) (V:=heap_cell) l (DfracOwn 1) (Storing v%V))
+Notation "l ↦ v" := (mapsto (L:=loc) (V:=val) l (DfracOwn 1) (v%V))
   (at level 20, format "l  ↦  v") : bi_scope.
-Notation "l ↦{ dq } '?'" := (mapsto (L:=loc) (V:=heap_cell) l dq (Uninitialized))
-  (at level 20, format "l  ↦{ dq }  ?") : bi_scope.
-Notation "l ↦□ '?'" := (mapsto (L:=loc) (V:=heap_cell) l DfracDiscarded (Uninitialized))
-  (at level 20, format "l  ↦□  ?") : bi_scope.
-Notation "l ↦{# q } '?'" := (mapsto (L:=loc) (V:=heap_cell) l (DfracOwn q) (Uninitialized))
-  (at level 20, format "l  ↦{# q }  ?") : bi_scope.
-Notation "l ↦ '?'" := (mapsto (L:=loc) (V:=heap_cell) l (DfracOwn 1) (Uninitialized))
-  (at level 20, format "l  ↦  ?") : bi_scope.
 
 (** Same for [gen_inv_heap], except that these are higher-order notations so to
 make setoid rewriting in the predicate [I] work we need actual definitions
 here. *)
 Section definitions.
-  Context `{!heapGS Σ}.
-
-  Definition from_storing (I : val → Prop) (Puninit Pfree : Prop) (k : heap_cell) :=
-    match k with
-    | None => Pfree
-    | Some None => Puninit
-    | Some (Some v) => I v
-    end.
-
+  Context `{!heapGS_gen hlc Σ}.
   Definition inv_mapsto_own (l : loc) (v : val) (I : val → Prop) : iProp Σ :=
-    inv_mapsto_own l (Storing v) (from_storing I False False).
+    inv_mapsto_own l v I.
   Definition inv_mapsto (l : loc) (I : val → Prop) : iProp Σ :=
-    inv_mapsto l (from_storing I False False).
+    inv_mapsto l I.
 End definitions.
 
 Global Instance: Params (@inv_mapsto_own) 4 := {}.
 Global Instance: Params (@inv_mapsto) 3 := {}.
 
-Notation inv_heap_inv := (inv_heap_inv loc heap_cell).
+Notation inv_heap_inv := (inv_heap_inv loc val).
 Notation "l '↦_' I □" := (inv_mapsto l I%stdpp%type)
   (at level 20, I at level 9, format "l  '↦_' I  '□'") : bi_scope.
 Notation "l ↦_ I v" := (inv_mapsto_own l v I%stdpp%type)
   (at level 20, I at level 9, format "l  ↦_ I  v") : bi_scope.
 
 Section lifting.
-Context `{!heapGS Σ}.
-Context {p:prog_environ}.
+Context `{!heapGS_gen hlc Σ}.
 Implicit Types P Q : iProp Σ.
 Implicit Types Φ Ψ : val → iProp Σ.
 Implicit Types efs : list expr.
 Implicit Types σ : state.
 Implicit Types v : val.
 Implicit Types l : loc.
-
-(*
-#[global] Instance wp'': Wp (iProp Σ) expr val stuckness := (@wp' (C_lang p) Σ _).
-#[global] Instance twp'': Twp (iProp Σ) expr val stuckness := (@twp' (C_lang p) Σ _).
-*)
+Implicit Types s : prog_environ.
 
 Lemma wp_lb_init s E e Φ :
   TCEq (to_val e) None →
@@ -199,23 +160,22 @@ Qed.
 (** Recursive functions: we do not use this lemmas as it is easier to use Löb
 induction directly, but this demonstrates that we can state the expected
 reasoning principle for recursive functions, without any visible ▷. *)
-Lemma wp_rec_löb s E f e args Φ (Ψ : list val → iProp Σ) :
-   ⌜(weakestpre.prog s) !! f = Some (Fun args e)⌝ -∗
-  □ ( □ (∀ vs res, Ψ vs -∗ ⌜zip_args args vs = Some res⌝ -∗ WP (FunCall ((&f)%V) (map Val vs)) @ s; E {{ Φ }}) -∗
-     ∀ vs res, Ψ vs -∗ ⌜zip_args args vs = Some res⌝ -∗ WP (subst_all res e) @ s; E {{ Φ }}) -∗
-  ∀ vs res , Ψ vs -∗ ⌜zip_args args vs = Some res⌝ -∗ WP (FunCall ((&f)%V) (map Val vs)) @ s; E {{ Φ }}.
+Lemma wp_rec_löb s E f x e Φ Ψ :
+  □ ( □ (∀ v, Ψ v -∗ WP (rec: f x := e)%V v @ s; E {{ Φ }}) -∗
+     ∀ v, Ψ v -∗ WP (subst' x v (subst' f (rec: f x := e) e)) @ s; E {{ Φ }}) -∗
+  ∀ v, Ψ v -∗ WP (rec: f x := e)%V v @ s; E {{ Φ }}.
 Proof.
-  iIntros "%Hp #Hrec". iLöb as "IH". iIntros (v res) "HΨ %Hres".
-  iApply lifting.wp_pure_step_later; first apply pure_funcall. 1: eauto.
-  iIntros "!>". iApply ("Hrec" with "[] HΨ"). 2:done. iIntros "!>" (w res') "HΨ %Hres'".
-  iApply ("IH" with "HΨ"). iPureIntro. apply Hres'.
+  iIntros "#Hrec". iLöb as "IH". iIntros (v) "HΨ".
+  iApply lifting.wp_pure_step_later; first apply pure_beta. 2: eauto.
+  1: apply as_recv.
+  iIntros "!>". iApply ("Hrec" with "[] HΨ"). iIntros "!>" (w) "HΨ".
+  iApply ("IH" with "HΨ").
 Qed.
-
 
 (** Heap *)
 
 (** We need to adjust the [gen_heap] and [gen_inv_heap] lemmas because of our
-value type being [option val]. *)
+value type being [val]. *)
 
 Lemma mapsto_valid l dq v : l ↦{dq} v -∗ ⌜✓ dq⌝.
 Proof. apply mapsto_valid. Qed.
@@ -246,14 +206,12 @@ Proof. apply mapsto_persist. Qed.
 Global Instance inv_mapsto_own_proper l v :
   Proper (pointwise_relation _ iff ==> (≡)) (inv_mapsto_own l v).
 Proof.
-  intros I1 I2 HI. rewrite /inv_mapsto_own. f_equiv=>-[[w|]|]; [|done|done].
-  simpl. apply HI.
+  intros I1 I2 HI. rewrite /inv_mapsto_own. f_equiv; done.
 Qed.
 Global Instance inv_mapsto_proper l :
   Proper (pointwise_relation _ iff ==> (≡)) (inv_mapsto l).
 Proof.
-  intros I1 I2 HI. rewrite /inv_mapsto. f_equiv=>-[[w|]|]; [|done|done].
-  simpl. apply HI.
+  intros I1 I2 HI. rewrite /inv_mapsto. f_equiv; done.
 Qed.
 
 Lemma make_inv_mapsto l v (I : val → Prop) E :
@@ -273,7 +231,7 @@ Proof.
   iIntros (?) "#Hinv".
   iMod (inv_mapsto_own_acc_strong with "Hinv") as "Hacc"; first done.
   iIntros "!>" (l v I) "Hl". iDestruct ("Hacc" with "Hl") as "(% & Hl & Hclose)".
-  iFrame "%∗". iIntros (w) "% Hl". iApply "Hclose"; done.
+  iFrame "%∗".
 Qed.
 
 Lemma inv_mapsto_own_acc E l v I:
@@ -283,7 +241,7 @@ Lemma inv_mapsto_own_acc E l v I:
 Proof.
   iIntros (?) "#Hinv Hl".
   iMod (inv_mapsto_own_acc with "Hinv Hl") as "(% & Hl & Hclose)"; first done.
-  iFrame "%∗". iIntros "!>" (w) "% Hl". iApply "Hclose"; done.
+  iFrame "%∗". by iModIntro.
 Qed.
 
 Lemma inv_mapsto_acc l I E :
@@ -292,7 +250,7 @@ Lemma inv_mapsto_acc l I E :
     ∃ v, ⌜I v⌝ ∗ l ↦ v ∗ (l ↦ v ={E ∖ ↑inv_heapN, E}=∗ ⌜True⌝).
 Proof.
   iIntros (?) "#Hinv Hl".
-  iMod (inv_mapsto_acc with "Hinv Hl") as ([[v|]|]) "(% & Hl & Hclose)"; [done| |done|done].
+  iMod (inv_mapsto_acc with "Hinv Hl") as (v) "(% & Hl & Hclose)"; [done|].
   iIntros "!>". iExists (v). iFrame "%∗".
 Qed.
 
@@ -306,7 +264,7 @@ Proof.
   iIntros (<-) "Hvs". iInduction vs as [|v vs] "IH" forall (l)=> //=.
   rewrite big_opM_union; last first.
   { apply map_disjoint_spec=> l' v1 v2 /lookup_singleton_Some [-> _].
-    intros (j&?&Hjl&?)%heap_array_lookup.
+    intros (j&w&Hjl&?)%heap_array_lookup.
     rewrite loc_add_assoc -{1}[l']loc_add_0 in Hjl. simplify_eq; lia. }
   rewrite loc_add_0 -fmap_S_seq big_sepL_fmap.
   setoid_rewrite Nat2Z.inj_succ. setoid_rewrite <-Z.add_1_l.
@@ -314,15 +272,15 @@ Proof.
   rewrite big_opM_singleton; iDestruct "Hvs" as "[$ Hvs]". by iApply "IH".
 Qed.
 
-Lemma heap_array_to_seq_mapsto l (v:heap_cell) (n : nat) :
+Lemma heap_array_to_seq_mapsto l v (n : nat) :
   ([∗ map] l' ↦ ov ∈ heap_array l (replicate n v), gen_heap.mapsto l' (DfracOwn 1) ov) -∗
-  [∗ list] i ∈ seq 0 n, (l +ₗ (i : nat)) O↦ v.
+  [∗ list] i ∈ seq 0 n, (l +ₗ (i : nat)) ↦ v.
 Proof.
   iIntros "Hvs". iInduction n as [|n] "IH" forall (l); simpl.
   { done. }
   rewrite big_opM_union; last first.
   { apply map_disjoint_spec=> l' v1 v2 /lookup_singleton_Some [-> _].
-    intros (j&?&Hjl&_)%heap_array_lookup.
+    intros (j&w&Hjl&_)%heap_array_lookup.
     rewrite loc_add_assoc -{1}[l']loc_add_0 in Hjl. simplify_eq; lia. }
   rewrite loc_add_0 -fmap_S_seq big_sepL_fmap.
   setoid_rewrite Nat2Z.inj_succ. setoid_rewrite <-Z.add_1_l.
@@ -330,16 +288,16 @@ Proof.
   rewrite big_opM_singleton; iDestruct "Hvs" as "[$ Hvs]". by iApply "IH".
 Qed.
 
-Lemma wp_Malloc_seq E n :
+Lemma wp_allocN_seq s E v n :
   (0 < n)%Z →
-  {{{ True }}} Malloc (Val $ LitV $ LitInt $ n) @ p; E
+  {{{ True }}} AllocN (Val $ LitV $ LitInt $ n) (Val v) @ s; E
   {{{ l, RET LitV (LitLoc l); [∗ list] i ∈ seq 0 (Z.to_nat n),
-      (l +ₗ (i : nat)) ↦ ? ∗ meta_token (l +ₗ (i : nat)) ⊤ }}}.
+      (l +ₗ (i : nat)) ↦ v ∗ meta_token (l +ₗ (i : nat)) ⊤ }}}.
 Proof.
   iIntros (Hn Φ) "_ HΦ". iApply wp_lift_atomic_head_step; first done.
-  iIntros (σ1 ns) "(Hσ & Hsteps)". iModIntro. iSplit; first (destruct n; eauto with lia head_step).
-  iIntros (e2 σ2 Hstep). inv_head_step. iModIntro.
-  iMod (gen_heap_alloc_big _ (heap_array _ (replicate (Z.to_nat n) Uninitialized)) with "Hσ")
+  iIntros (σ1 ns) "(Hσ & Hsteps)". iModIntro. iSplit; first (destruct n; eauto with lia head_step).  
+  iIntros (v2 σ2 Hstep). inv_head_step. iModIntro.
+  iMod (gen_heap_alloc_big _ (heap_array _ (replicate (Z.to_nat n) v)) with "Hσ")
     as "(Hσ & Hl & Hm)".
   { apply heap_array_map_disjoint.
     rewrite replicate_length Z2Nat.id; auto with lia. }
@@ -350,49 +308,75 @@ Proof.
   - iApply (heap_array_to_seq_meta with "Hm"). by rewrite replicate_length.
 Qed.
 
-Lemma wp_free s E l (v:option val) :
-  {{{ ▷ l O↦ Some v}}} Free (Val $ LitV $ LitLoc l) (Val $ LitV $ LitInt 1) @ s; E
-  {{{ RET LitV LitUnit; True }}}.
+Lemma wp_alloc s E v :
+  {{{ True }}} Alloc (Val v) @ s; E {{{ l, RET LitV (LitLoc l); l ↦ v ∗ meta_token l ⊤ }}}.
 Proof.
-  iIntros (Φ) ">Hl HΦ". iApply (wp_step with "HΦ"). iApply wp_lift_atomic_head_step; first done.
-  iIntros (σ1 ns) "(Hσ & Hsteps) !>". iDestruct (gen_heap_valid with "Hσ Hl") as %?.
-  iSplit; first by eauto with head_step.
-  iIntros (e2 σ2 Hstep); inv_head_step.
-  rewrite state_init_heap_singleton. iModIntro.
-  iMod (gen_heap_update (σ1) l (Some v) Deallocated with "Hσ Hl") as "[$ Hl]".
-  iMod (steps_auth_update_S with "Hsteps") as "Hsteps".
-  iModIntro. iFrame. iIntros "HΦ". iModIntro. by iApply "HΦ".
+  iIntros (Φ) "_ HΦ". iApply wp_allocN_seq; [auto with lia..|]. iModIntro.
+  iIntros (l) "/= (? & _)". rewrite loc_add_0. iApply "HΦ"; iFrame.
 Qed.
 
+(*
+Lemma swp_free s E l v :
+  {{{ l ↦ v }}} Free (Val $ LitV $ LitLoc l) @ s; E
+  {{{ RET LitV LitUnit; True }}}.
+Proof.
+  iIntros (Φ) "Hl HΦ". iApply twp_lift_atomic_head_step_no_fork; first done.
+  iIntros (σ1 ns κs nt) "(Hσ & Hsteps) !>". iDestruct (gen_heap_valid with "Hσ Hl") as %?.
+  iSplit; first by eauto with head_step.
+  iIntros (κ v2 σ2 efs Hstep); inv_head_step.
+  iMod (gen_heap_update with "Hσ Hl") as "[$ Hl]".
+  iMod (steps_auth_update_S with "Hsteps") as "Hsteps".
+  iModIntro. iSplit; first done. iSplit; first done. iFrame. by iApply "HΦ".
+Qed.
+Lemma wp_free s E l v :
+  {{{ ▷ l ↦ v }}} Free (Val $ LitV (LitLoc l)) @ s; E
+  {{{ RET LitV LitUnit; True }}}.
+Proof.
+  iIntros (Φ) ">H HΦ". iApply (twp_wp_step with "HΦ").
+  iApply (twp_free with "H"); [by auto..|]; iIntros "H HΦ". by iApply "HΦ".
+Qed. *)
+
+Lemma wp_load' s E l dq v :
+  {{{ l ↦{dq} v }}} Load (Val $ LitV $ LitLoc l) @ s; E {{{ RET v; l ↦{dq} v }}}.
+Proof.
+  iIntros (Φ) "Hl HΦ". iApply wp_lift_atomic_head_step; first done.
+  iIntros (σ1 ns) "(Hσ & Hsteps) !>". iDestruct (gen_heap_valid with "Hσ Hl") as %?.
+  iSplit; first by eauto with head_step. iModIntro.
+  iIntros (v2 σ2 Hstep); inv_head_step.
+  iMod (steps_auth_update_S with "Hsteps") as "Hsteps". iFrame.
+  by iApply "HΦ".
+Qed.
 Lemma wp_load s E l dq v :
   {{{ ▷ l ↦{dq} v }}} Load (Val $ LitV $ LitLoc l) @ s; E {{{ RET v; l ↦{dq} v }}}.
 Proof.
-  iIntros (Φ) "> Hl HΦ". iApply (wp_step with "HΦ"). iApply wp_lift_atomic_head_step; first done.
-  iIntros (σ1 ns) "(Hσ & Hsteps)". iDestruct (gen_heap_valid with "Hσ Hl") as "%HH". iModIntro.
-  iSplitR; first ( iPureIntro; eauto with head_step).
-  iIntros (e2 σ2 Hstep); inv_head_step. iModIntro.
-  iMod (steps_auth_update_S with "Hsteps") as "Hsteps".
-  iModIntro. iFrame. iIntros "HΦ". iModIntro.
-  by iApply "HΦ".
+  iIntros (Φ) ">Hl HΦ". iApply (wp_step with "HΦ").
+  iApply (wp_load' with "Hl"). iIntros "!> H HΦ". by iApply "HΦ".
 Qed.
 
-Lemma wp_store s E l (v':option val) v :
-  {{{ ▷ l O↦ Some v' }}} Store (Val $ LitV $ LitLoc l) (Val v) @ s; E
+Lemma wp_store' s E l v' v :
+  {{{ l ↦ v' }}} Store (Val $ LitV $ LitLoc l) (Val v) @ s; E
   {{{ RET LitV LitUnit; l ↦ v }}}.
 Proof.
-  iIntros (Φ) "> Hl HΦ". iApply (wp_step with "HΦ"). iApply wp_lift_atomic_head_step; first done.
+  iIntros (Φ) "Hl HΦ". iApply wp_lift_atomic_head_step; first done.
   iIntros (σ1 ns) "(Hσ & Hsteps) !>". iDestruct (gen_heap_valid with "Hσ Hl") as %?.
   iSplit; first by eauto with head_step.
-  iIntros (e2 σ2 Hstep); inv_head_step. iModIntro.
+  iIntros (v2 σ2 Hstep); inv_head_step. iModIntro.
   iMod (steps_auth_update_S with "Hsteps") as "Hsteps".
   iMod (gen_heap_update with "Hσ Hl") as "[$ Hl]".
-  iModIntro. iFrame. iIntros "HΦ". iModIntro. by iApply "HΦ".
+  iModIntro. iFrame. by iApply "HΦ".
+Qed.
+Lemma wp_store s E l v' v :
+  {{{ ▷ l ↦ v' }}} Store (Val $ LitV (LitLoc l)) (Val v) @ s; E
+  {{{ RET LitV LitUnit; l ↦ v }}}.
+Proof.
+  iIntros (Φ) ">H HΦ". iApply (wp_step with "HΦ").
+  iApply (wp_store' with "H"). iIntros "!> H HΦ". by iApply "HΦ".
 Qed.
 
 (*
 Lemma twp_xchg s E l v' v :
-  [[{ l ↦ v' }]] Xchg (Val $ LitV $ LitLoc l) (Val v) @ s; E
-  [[{ RET v'; l ↦ v }]].
+  {{{ l ↦ v' }}} Xchg (Val $ LitV $ LitLoc l) (Val v) @ s; E
+  {{{ RET v'; l ↦ v }}}.
 Proof.
   iIntros (Φ) "Hl HΦ". iApply twp_lift_atomic_head_step_no_fork; first done.
   iIntros (σ1 ns κs nt) "(Hσ & Hκs & Hsteps) !>". iDestruct (gen_heap_valid with "Hσ Hl") as %?.
@@ -412,8 +396,8 @@ Qed.
 
 Lemma twp_cmpxchg_fail s E l dq v' v1 v2 :
   v' ≠ v1 → vals_compare_safe v' v1 →
-  [[{ l ↦{dq} v' }]] CmpXchg (Val $ LitV $ LitLoc l) (Val v1) (Val v2) @ s; E
-  [[{ RET PairV v' (LitV $ LitBool false); l ↦{dq} v' }]].
+  {{{ l ↦{dq} v' }}} CmpXchg (Val $ LitV $ LitLoc l) (Val v1) (Val v2) @ s; E
+  {{{ RET PairV v' (LitV $ LitBool false); l ↦{dq} v' }}}.
 Proof.
   iIntros (?? Φ) "Hl HΦ". iApply twp_lift_atomic_head_step_no_fork; first done.
   iIntros (σ1 ns κs nt) "(Hσ & Hκs & Hsteps) !>". iDestruct (gen_heap_valid with "Hσ Hl") as %?.
@@ -434,8 +418,8 @@ Qed.
 
 Lemma twp_cmpxchg_suc s E l v1 v2 v' :
   v' = v1 → vals_compare_safe v' v1 →
-  [[{ l ↦ v' }]] CmpXchg (Val $ LitV $ LitLoc l) (Val v1) (Val v2) @ s; E
-  [[{ RET PairV v' (LitV $ LitBool true); l ↦ v2 }]].
+  {{{ l ↦ v' }}} CmpXchg (Val $ LitV $ LitLoc l) (Val v1) (Val v2) @ s; E
+  {{{ RET PairV v' (LitV $ LitBool true); l ↦ v2 }}}.
 Proof.
   iIntros (?? Φ) "Hl HΦ". iApply twp_lift_atomic_head_step_no_fork; first done.
   iIntros (σ1 ns κs nt) "(Hσ & Hκs & Hsteps) !>". iDestruct (gen_heap_valid with "Hσ Hl") as %?.
@@ -456,8 +440,8 @@ Proof.
 Qed.
 
 Lemma twp_faa s E l i1 i2 :
-  [[{ l ↦ LitV (LitInt i1) }]] FAA (Val $ LitV $ LitLoc l) (Val $ LitV $ LitInt i2) @ s; E
-  [[{ RET LitV (LitInt i1); l ↦ LitV (LitInt (i1 + i2)) }]].
+  {{{ l ↦ LitV (LitInt i1) }}} FAA (Val $ LitV $ LitLoc l) (Val $ LitV $ LitInt i2) @ s; E
+  {{{ RET LitV (LitInt i1); l ↦ LitV (LitInt (i1 + i2)) }}}.
 Proof.
   iIntros (Φ) "Hl HΦ". iApply twp_lift_atomic_head_step_no_fork; first done.
   iIntros (σ1 ns κs nt) "(Hσ & Hκs & Hsteps) !>". iDestruct (gen_heap_valid with "Hσ Hl") as %?.
@@ -482,7 +466,7 @@ Lemma wp_new_proph s E :
 Proof.
   iIntros (Φ) "_ HΦ". iApply wp_lift_atomic_head_step_no_fork; first done.
   iIntros (σ1 ns κ κs nt) "(Hσ & HR & Hsteps) !>". iSplit; first by eauto with head_step.
-  iIntros "!>" (v2 σ2 efs Hstep). inv_head_step.
+  iIntros "!>" (v2 σ2 efs Hstep) "_". inv_head_step.
   rename select proph_id into p.
   iMod (steps_auth_update_S with "Hsteps") as "Hsteps".
   iMod (proph_map_new_proph p with "HR") as "[HR Hp]"; first done.
@@ -551,9 +535,9 @@ Proof.
   - rewrite -assoc.
     iMod ("WPe" $! σ1 ns _ _ nt with "[$Hσ $Hκ $Hsteps]") as "[Hs WPe]". iModIntro. iSplit.
     { iDestruct "Hs" as %?. iPureIntro. destruct s; [ by apply resolve_reducible | done]. }
-    iIntros (e2 σ2 efs step). apply step_resolve in step; last done.
+    iIntros (e2 σ2 efs step) "Hcred". apply step_resolve in step; last done.
     inv_head_step; simplify_list_eq.
-    iMod ("WPe" $! (Val w') σ2 efs with "[%]") as "WPe".
+    iMod ("WPe" $! (Val w') σ2 efs with "[%] Hcred") as "WPe".
     { by eexists [] _ _. }
     iModIntro. iNext. iMod "WPe" as "WPe". iModIntro.
     iApply (step_fupdN_wand with "WPe"); iIntros "> [($ & Hκ & $) WPe]".
