theories/ml_toy_lang/iris/derived_laws.v
@@ -7,8 +7,8 @@ For utility functions on arrays (e.g., freeing/copying an array), see
 From stdpp Require Import fin_maps.
 From iris.bi Require Import lib.fractional.
 From iris.proofmode Require Import proofmode.
-From melocoton.ml_toy_lang Require Export primitive_laws.
-From melocoton.ml_toy_lang Require Import tactics notation.
+From melocoton.ml_toy_lang Require Export iris.primitive_laws.
+From melocoton.ml_toy_lang Require Import iris.tactics notation.
 From iris.prelude Require Import options.
 
 (** The [array] connective is a version of [mapsto] that works
