theories/ml_toy_lang/melocoton/class_instances.v
@@ -1,0 +1,105 @@
+From melocoton.language Require Export language weakestpre lifting.
+From melocoton.ml_toy_lang Require Export melocoton.lang_instantiation lang.
+From melocoton.ml_toy_lang Require Import tactics melocoton.tactics notation lang.
+From iris.prelude Require Import options.
+Import ml_toy_lang.
+
+(** * Instances of the [PureExec] class *)
+(** The behavior of the various [wp_] tactics with regard to lambda differs in
+the following way:
+
+- [wp_pures] does *not* reduce lambdas/recs that are hidden behind a definition.
+- [wp_rec] and [wp_lam] reduce lambdas/recs that are hidden behind a definition.
+
+To realize this behavior, we define the class [AsRecV v f x erec], which takes a
+value [v] as its input, and turns it into a [RecV f x erec] via the instance
+[AsRecV_recv : AsRecV (RecV f x e) f x e]. We register this instance via
+[Hint Extern] so that it is only used if [v] is syntactically a lambda/rec, and
+not if [v] contains a lambda/rec that is hidden behind a definition.
+
+To make sure that [wp_rec] and [wp_lam] do reduce lambdas/recs that are hidden
+behind a definition, we activate [AsRecV_recv] by hand in these tactics. *)
+
+Class AsRecV (v : val) (f x : binder) (erec : expr) :=
+  as_recv : v = RecV f x erec.
+Global Hint Mode AsRecV ! - - - : typeclass_instances.
+Definition AsRecV_recv f x e : AsRecV (RecV f x e) f x e := eq_refl.
+Global Hint Extern 0 (AsRecV (RecV _ _ _) _ _ _) =>
+  apply AsRecV_recv : typeclass_instances.
+
+Section pure_exec.
+  Context  {p:ml_program}.
+  Local Ltac solve_exec_safe := intros; subst; do 3 eexists; try (repeat (econstructor; eauto); done).
+  Local Ltac solve_exec_puredet := simpl; intros; inv_head_step; try inv_head_step; try done.
+  Local Ltac solve_pure_exec :=
+    subst; intros ?; apply nsteps_once, pure_head_step_pure_step;
+      constructor; [solve_exec_safe | solve_exec_puredet].
+
+  Global Instance pure_recc f x (erec : expr) :
+    PureExec True 1 p (Rec f x erec) (Val $ RecV f x erec).
+  Proof. solve_pure_exec. Qed.
+  Global Instance pure_pairc (v1 v2 : val) :
+    PureExec True 1 p (Pair (Val v1) (Val v2)) (Val $ PairV v1 v2).
+  Proof. solve_pure_exec. Qed.
+  Global Instance pure_injlc (v : val) :
+    PureExec True 1 p (InjL $ Val v) (Val $ InjLV v).
+  Proof. solve_pure_exec. Qed.
+  Global Instance pure_injrc (v : val) :
+    PureExec True 1 p (InjR $ Val v) (Val $ InjRV v).
+  Proof. solve_pure_exec. Qed.
+
+  Global Instance pure_beta f x (erec : expr) (v1 v2 : val) `{!AsRecV v1 f x erec} :
+    PureExec True 1 p (App (Val v1) (Val v2)) (subst' x v2 (subst' f v1 erec)).
+  Proof. unfold AsRecV in *. solve_pure_exec. Qed.
+
+  Global Instance pure_unop op v v' :
+    PureExec (un_op_eval op v = Some v') 1 p (UnOp op (Val v)) (Val v').
+  Proof. solve_pure_exec. Qed.
+
+  Global Instance pure_binop op v1 v2 v' :
+    PureExec (bin_op_eval op v1 v2 = Some v') 1 p (BinOp op (Val v1) (Val v2)) (Val v') | 10.
+  Proof. solve_pure_exec. Qed.
+  (* Lower-cost instance for [EqOp]. *)
+  Global Instance pure_eqop v1 v2 :
+    PureExec (vals_compare_safe v1 v2) 1 p
+      (BinOp EqOp (Val v1) (Val v2))
+      (Val $ LitV $ LitBool $ bool_decide (v1 = v2)) | 1.
+  Proof.
+    intros Hcompare.
+    cut (bin_op_eval EqOp v1 v2 = Some $ LitV $ LitBool $ bool_decide (v1 = v2)).
+    { intros. revert Hcompare. solve_pure_exec. }
+    rewrite /bin_op_eval /= decide_True //.
+  Qed.
+
+  Global Instance pure_if_true e1 e2 :
+    PureExec True 1 p (If (Val $ LitV $ LitBool true) e1 e2) e1.
+  Proof. solve_pure_exec. Qed.
+  Global Instance pure_if_false e1 e2 :
+    PureExec True 1 p (If (Val $ LitV  $ LitBool false) e1 e2) e2.
+  Proof. solve_pure_exec. Qed.
+
+  Global Instance pure_fst v1 v2 :
+    PureExec True 1 p (Fst (Val $ PairV v1 v2)) (Val v1).
+  Proof. solve_pure_exec. Qed.
+  Global Instance pure_snd v1 v2 :
+    PureExec True 1 p (Snd (Val $ PairV v1 v2)) (Val v2).
+  Proof. solve_pure_exec. Qed.
+
+  Global Instance pure_case_inl v e1 e2 :
+    PureExec True 1 p (Case (Val $ InjLV v) e1 e2) (App e1 (Val v)).
+  Proof. solve_pure_exec. Qed.
+  Global Instance pure_case_inr v e1 e2 :
+    PureExec True 1 p (Case (Val $ InjRV v) e1 e2) (App e2 (Val v)).
+  Proof. solve_pure_exec. Qed.
+  Global Instance pure_funcall s va f res : 
+    PureExec ((p : gmap.gmap string ml_function) !! s = Some f ∧ apply_function f va = Some res) 1 p (Extern s (map Val va)) res.
+  Proof. destruct f.
+         subst; intros ?; apply nsteps_once, pure_head_step_pure_step;
+         constructor; [solve_exec_safe | solve_exec_puredet].
+         + econstructor. destruct H. econstructor; done.
+         + repeat split; try congruence. destruct H as [H1 H2]. rewrite H3 in H1.
+           assert (args = b) as -> by congruence.
+           assert (e = e0) as -> by congruence.
+           congruence.
+  Qed.
+End pure_exec.
